specs/verif_hmac_drbg_update.v
@@ -1,0 +1,16 @@
+Require Import floyd.proofauto.
+Import ListNotations.
+Local Open Scope logic.
+Require Import sublist.
+
+Require Import hmac_drbg.
+Require Import spec_hmac_drbg.
+
+Lemma body_hmac_drbg_update: semax_body HmacDrbgVarSpecs HmacDrbgFunSpecs 
+       f_mbedtls_hmac_drbg_update hmac_drbg_update_spec.
+Proof.
+  start_function.
+  name ctx' _ctx.
+  name add_len' _add_len.
+  name additional' _additional.
+  forward.
